Start relation for evaluation rules of expressions

proof-of-soundness/c-subset-syntax.v
@@ -9,7 +9,12 @@ Open Scope string_scope.
 
 
 (* I'm not sure if this is correct, but it seems to work *)
-Definition state : Set := list (string * Z).
+Definition environment : Set := list (string * nat).
+Definition state : Set := list (nat * Z).
+
+(* TODO: Make these meaningful *)
+Definition lookupE (x:string) (E:environment) : nat := 1.
+Definition lookupS (l:nat) (S:state) : Z := 1.
 
 
 Inductive unop : Type :=
@@ -26,40 +31,35 @@ Inductive const_expr : Type :=
   | ConstNum (z : Z)
   | ConstParenExpr (ce : const_expr)
   | ConstUnExpr (uo : unop) (ce : const_expr)
-  | ConstBinExpr (ce1 ce2 : const_expr) (bo : binop).
+  | ConstBinExpr (bo : binop) (ce1 ce2 : const_expr).
 
-Inductive var_expr : Type :=
+(* TODO: Currently we can only assign from strings to r-values.
+   This need to be fixed so that LHS of assignments can be an l-value *)
+Inductive expr : Type :=
   | X (x : string)
   | Num (z : Z)
-  | ParenExpr (va : var_expr)
-  | UnExpr (uo : unop) (va : var_expr)
-  | BinExpr (va1 va2 : var_expr) (bo : binop)
-  | Assign (va1 va2 : var_expr)
-  | CallOrInvoke (x : string) (vas: list var_expr).
-
-Inductive expr : Type :=
-  | ConstExpr (ce : const_expr)
-  | VarExpr (va : var_expr).
-
-(* TODO: Make this meaningful*)
-Definition lookup (x:string) : Z := 1.
+  | ParenExpr (e : expr)
+  | UnExpr (uo : unop) (e : expr)
+  | BinExpr (bo : binop) (e1 e2 : expr)
+  | Assign (x: string) (e : expr)
+  | CallOrInvoke (x : string) (es: list expr).
 
 (* TODO: Add state to these evaluation rules.
    May have to define evaluation as a relation instead of as
    a function *)
-Fixpoint ceval (ce : const_expr) : Z :=
+Fixpoint ceeval (ce : const_expr) : Z :=
   match ce with
   | ConstNum z => z
-  | ConstParenExpr ce => ceval ce
+  | ConstParenExpr ce => ceeval ce
   | ConstUnExpr uo ce =>
-    let v := ceval ce in
+    let v := ceeval ce in
       match uo with
      | Positive => id v
      | Negative => - v
      end
-  | ConstBinExpr ce1 ce2 bo =>
-    let v1 := (ceval ce1) in
-    let v2 := (ceval ce2) in
+  | ConstBinExpr bo ce1 ce2 =>
+    let v1 := (ceeval ce1) in
+    let v2 := (ceeval ce2) in
       match bo with
       | Plus => v1 + v2
       | Sub => v1 - v2
@@ -68,41 +68,95 @@ Fixpoint ceval (ce : const_expr) : Z :=
       end
 end.
 
-
-Fixpoint veval (va : var_expr) : Z :=
-  match va with
-  | X x => lookup x
+Fixpoint eeval (e : expr) : Z :=
+  match e with
+  | X x => 0
   | Num n => n
-  | ParenExpr va => veval va
-  | UnExpr uo va =>
-    let v := veval va in
+  | ParenExpr e => eeval e
+  | UnExpr uo e =>
+    let v := eeval e in
       match uo with
       | Positive => id v
       | Negative => - v
       end
-  | BinExpr va1 va2 bo =>
-    let v1 := veval va1 in
-    let v2 := veval va2 in
+  | BinExpr bo e1 e2 =>
+    let v1 := eeval e1 in
+    let v2 := eeval e2 in
       match bo with
       | Plus => v1 + v2
       | Sub => v1 - v2
       | Mul => v1 * v2
       | Div => v1 / v2
       end
-  | Assign va1 va2 => 
+  | Assign x e => 
     (* TODO: Return the update to the state! *)
-    veval va2
+    eeval e
   | CallOrInvoke x vas =>
     (* TODO: Add semantics for function calls and invocations*)
     0
   end.
 
-
-Definition eeval (e : expr) : Z :=
-  match e with
-  | ConstExpr ce => ceval ce
-  | VarExpr va => veval va
-  end.
+Reserved Notation
+  "[ S , E '|-' e '=>' v , S' ]"
+  (at level 90, left associativity).
+Inductive eevalR : state -> environment -> expr -> Z -> state -> Prop :=
+  (* Variable lookup returns the variable's r-value
+     and does not change the state *)
+  | E_X : forall S E x l v,
+    lookupE x E = l ->
+    lookupS l S = v ->
+    [S, E |- (X x) => v, S]
+  (* Numerals evaluate to their integer representation and do not
+     change the state *)
+  | E_Num : forall S E n,
+    [S, E |- (Num n) => n, S]
+  (* Parenthesized expressions evaluate to themselves.
+     Currently they do not change the state, but TODO: fix this *)
+  | E_ParenExpr : forall S E e v S',
+    [S, E |- e => v, S'] ->
+    [S, E |- (ParenExpr e) => v, S']
+  (* Unary negation evaluates the inner expression, and returns
+     the negation of that result along with any side-effects
+     from evaluating it*)
+  | E_UnExprNegate : forall S E S' e v,
+    [S, E |- e => v, S'] ->
+    [S', E |- (UnExpr Negative e) => -v, S']
+  (* Unary positive evaluates the inner expression, and returns
+     the that result along with any side-effects from evaluating it*)
+  | E_UnExprPositive : forall S E S' e v,
+    [S, E |- e => v, S'] ->
+    [S', E |- (UnExpr Positive e) => v, S']
+  (* Binary expressions evaluate their inner expressions
+     in left-to-right-order, apply their operator to these subresults,
+     and return the appropriate result along with any side-effects
+     that occurred from evaluating subexpressions. *)
+  (* NOTE: Evaluation rules do not handle operator precedence.
+     The parser must use a concrete syntax to generate a parse tree
+     with the appropriate precedence levels in it.*)
+  | E_BinExprPlus : forall S E S' S'' S''' e1 e2 v1 v2,
+    [S, E |- e1 => v1, S'] ->
+    [S', E |- e2 => v2, S''] ->
+    [S'', E |- (BinExpr Plus e1 e2) => (v1 + v2), S''']
+  | E_BinExprSub : forall S E S' S'' S''' e1 e2 v1 v2,
+    [S, E |- e1 => v1, S'] ->
+    [S', E |- e2 => v2, S''] ->
+    [S'', E |- (BinExpr Sub e1 e2) => (v1 - v2), S''']
+  | E_BinExprMul : forall S E S' S'' S''' e1 e2 v1 v2,
+    [S, E |- e1 => v1, S'] ->
+    [S', E |- e2 => v2, S''] ->
+    [S'', E |- (BinExpr Mul e1 e2) => (v1 * v2), S''']
+  | E_BinExprDiv : forall S E S' S'' S''' e1 e2 v1 v2,
+    [S, E |- e1 => v1, S'] ->
+    [S', E |- e2 => v2, S''] ->
+    [S'', E |- (BinExpr Div e1 e2) => (v1 / v2), S''']
+  | E_Assign : forall S E l x e v S' S'',
+    [S, E |- e => v, S'] ->
+    lookupE x E = l ->
+    (* TODO: Actually store the variable *)
+    (* update S' l v = S''*)
+    S'' = S' ->
+    [S, E |- (Assign x e) => v, S'']
+  where "[ S , E '|-' e '=>' v , S' ]" := (eevalR S E e v S') : type_scope.
 
 Lemma nnzeq : forall z : Z,
   - - z = z.
@@ -112,7 +166,7 @@ Proof. induction z as []; reflexivity. Qed.
 that applying the unary operation negate to a constant exprression twice
 results in the same value.*)
 Theorem neg_neg_equal_ce : forall ce : const_expr,
-  ceval (ConstUnExpr Negative (ConstUnExpr Negative ce)) = ceval ce.
+  ceeval (ConstUnExpr Negative (ConstUnExpr Negative ce)) = ceeval ce.
 Proof.
   induction ce as []; simpl; rewrite nnzeq; reflexivity.
 Qed.
@@ -120,7 +174,7 @@ Qed.
 (* Proof that adding zero any constant exprression results in the same
 value *)
 Theorem optimize_ce: forall ce : const_expr,
-  ceval (ConstBinExpr (ConstNum 0) ce Plus) = ceval ce.
+  ceeval (ConstBinExpr Plus (ConstNum 0) ce) = ceeval ce.
 Proof.
   induction ce as []; reflexivity.
 Qed.
@@ -144,11 +198,11 @@ Inductive stmt : Type :=
 
 Reserved Notation
   "st '=[' s ']=>' st'"
-  (at level 90, left associativity).
+  (at level 91, left associativity).
 (* Define the evaluation rule for statements as a
    relation instead of an inductive type to permite the non-
    determinism introduced by while loops *)
-Inductive stmtevalR : stmt -> state -> state -> Prop :=
+Inductive stmtevalR : state -> stmt -> state -> Prop :=
   (* A skip statement does not change the state *)
   | E_Skip : forall st,
     st =[ Skip ]=> st
@@ -181,4 +235,4 @@ Inductive stmtevalR : stmt -> state -> state -> Prop :=
     st =[ s0 ]=> st' ->
     st' =[ WhileStmt e s0 ]=> st'' ->
     st =[ WhileStmt e s0 ]=> st''
-  where "st '=[' s ']=>' st'" := (stmtevalR s st st') : type_scope.
+  where "st '=[' s ']=>' st'" := (stmtevalR st s st') : type_scope.
